
---

## Technical Change

A firm uses capital $K$ and labor $L$ to produce output via CES production

$$
f(L, K) = [(A_L L)^\rho + (A_K K)^\rho]^\frac{1}{\rho}
$$

where $A_L$ is the productivity of labor, and $A_K$ is the productivity of capital and $\rho \in (-\infty, 1)$. Suppose the input price for labor is $w$ (for "wage") and the input price for capital is $r$ (for "rent"). Suppose a firm wishes to find the cheapest way to produce output $q$, and that this cost minimization problem has an internal solution (so we can ignore boundary constraints).

**(a) Solve for the cost-minimizing labor-capital ratio of the firm, $(L/K)$.**

Defining:

$$
q = \frac{Q}{K}
$$

$$
q = \frac{1}{K}[(A_L L)^\rho + (A_K K)^\rho]^\frac{1}{\rho}
$$

$$
q = [\left(\frac{1}{K}\right)^\rho\lbrace (A_L L)^\rho + (A_K K)^\rho\rbrace ]^\frac{1}{\rho}
$$

$$
q = [(A_L \frac{L}{K})^\rho + (A_K \frac{K}{K})^\rho]^\frac{1}{\rho}
$$

Transformed production function.

$$
q = [(A_L l)^\rho + A_K^\rho]^\frac{1}{\rho}
$$

Where $l = \frac{L}{K}$.

Cost function:

$$
C(K,L) = rK + wL
$$

Transformed cost function:

$$
c(l) = r + wl
$$

Profit per unit of capital:

$$
\hat \pi = q(l) - c(l)\\
\hat \pi = [(A_L l)^\rho + A_K^\rho]^\frac{1}{\rho} - r - wl
$$

First Order Condition:

$$
\frac{d\hat \pi}{dl} = 0 \implies \frac{d q}{dl} =  w
$$

$$
\frac{d}{dl} \left([(A_L l)^\rho + A_K^\rho]^\frac{1}{\rho}\right) = w
$$

$$
\frac{1}{\rho}[(A_L l)^\rho + A_K^\rho]^{\frac{1}{\rho} - 1}
\frac{d}{dl} \left((A_L l)^\rho + A_K^\rho\right) = w
$$

$$
\frac{1}{\rho}[(A_L l)^\rho + A_K^\rho]^\frac{1 - \rho}{\rho}
\left( \rho A_L^ \rho l^{\rho - 1} \right) = w
$$


$$
A_L^ \rho[(A_L l)^\rho + A_K^\rho]^{-\frac{\rho - 1}{\rho}}
  l^{\rho - 1} = w
$$

$$
[(A_L l)^\rho + A_K^\rho]^{-\frac{\rho - 1}{\rho}}
  l^{\rho - 1} = \frac{w}{A_L^\rho}
$$

$$
[(A_L l)^\rho + A_K^\rho]
l^{-\rho}
=
\left(\frac{w}{A_L^\rho} \right)^{-\frac{\rho}{\rho - 1}}
=
\left( \frac{A_L^\rho}{w} \right)^{\frac{\rho}{\rho - 1}}
$$

$$
A_L^\rho + \left( \frac{A_K}{l} \right)^\rho
=
\left( \frac{A_L^\rho}{w} \right)^{\frac{\rho}{\rho - 1}}
$$

$$
\left( \frac{A_K}{l} \right)^\rho
=
\left( \frac{A_L^\rho}{w} \right)^{\frac{\rho}{\rho - 1}} - A_L^\rho
$$

$$
\left( \frac{1}{l} \right)^\rho
=
\frac{1}{A_K^\rho} \left( \frac{A_L^\rho}{w} \right)^{\frac{\rho}{\rho - 1}} - \frac{A_L^\rho}{A_K^\rho}
$$

$$
l
=
\left(
\frac{1}{A_K^\rho} \left( \frac{A_L^\rho}{w} \right)^{\frac{\rho}{\rho - 1}} - \frac{A_L^\rho}{A_K^\rho}
\right)^{-\frac{1}{\rho}}
$$

>The optimal level of labor per capital is:
>$$
>l
>=
>\left(
>\frac{1}{A_K^\rho} \left( \frac{A_L^\rho}{w} \right)^{\frac{\rho}{\rho - 1}} - \frac{A_L^\rho}{A_K^\rho}
>\right)^{-\frac{1}{\rho}}
>$$

Where $l = L/K$.

**(b) When $\rho \rightarrow 0$, how does $(L/K)$ change with the input prices $(w, r)$ and the factor productivity $(A_L, A_K)$?**

To answer the question we have to analyze the limit:

$$
\lim_{\rho \to 0} l(\rho)
=
\lim_{\rho \to 0} \left(
\frac{1}{A_K^\rho} \left( \frac{A_L^\rho}{w} \right)^{\frac{\rho}{\rho - 1}} - \frac{A_L^\rho}{A_K^\rho}
\right)^{-\frac{1}{\rho}}
$$

$$
\lim_{\rho \to 0} l(\rho)
= 
(\frac{1}{1}\left( \frac{1}{w} \right)^0 - 1)^{-\infin}
=
\infin \implies \frac{L}{K} = \infin \implies K =0
$$

As $\rho$ approaches zero, the firm will optimize its profits by substituting all of its production factors with labor, meaning that labor is a perfect substitute for capital.

**(c) When $\rho > 0$ and $\rho < 0$, how does $(L/K)$ change with the input prices $(w, r)$ and the factor productivity $(A_L, A_K)$? Provide an intuition.**

 
$$
\lim_{\rho \to 1} l(\rho)
=
\lim_{\rho \to 1} \left(
\frac{1}{A_K^\rho} \left( \frac{A_L^\rho}{w} \right)^{\frac{\rho}{\rho - 1}} - \frac{A_L^\rho}{A_K^\rho}
\right)^{-\frac{1}{\rho}}
$$

$$
\lim_{\rho \to 1} l(\rho)
=
\left(
\frac{1}{A_K} \left( \frac{A_L}{w} \right)^\infin - \frac{A_L}{A_K}
\right)^{-1}
$$

If $A_L > w$
$$
\lim_{\rho \to 1} l(\rho)
= 0 \implies \frac{L}{K} = 0 \implies L = 0
$$

If $A_L = w$ and $A_L < 1$
$$
\lim_{\rho \to 1} l(\rho)
=
\left(
\frac{A_k}{1 - A_L}
\right)
$$


---

$$
\lim_{\rho \to -\infin} l(\rho)
=
\lim_{\rho \to -\infin} \left(
\frac{1}{A_K^\rho} \left( \frac{A_L^\rho}{w} \right)^{\frac{\rho}{\rho - 1}} - \frac{A_L^\rho}{A_K^\rho}
\right)^{-\frac{1}{\rho}}
$$

$$
\lim_{\rho \to -\infin} l(\rho)
=
\left(
\infin - \frac{A_L^\rho}{A_K^\rho}
\right)^{-\frac{1}{\rho}}
$$

$$
\lim_{\rho \to 1} l(\rho)
= 0 \implies \frac{L}{K} = 0 \implies L = 0
$$
