\section{General Equilibrium}

There are two goods and \( J \) agents, \( j \in \{1, \ldots, J\} \). Each agent has identical utility \( u(x^j_1, x^j_2) = \sqrt{x^j_1} + \sqrt{x^j_2} \). Agent \( j \) is endowed with \( (\omega^j_1, \omega^j_2) \). We normalize the price of good 2, so the prices of the two goods are \( (p_1, p_2) = (p, 1) \). Denote aggregate endowments by \( \omega_1 = \sum_j \omega^j_1 \) and \( \omega_2 = \sum_j \omega^j_2 \).


%%%%%%%%%%%%%%%%%%%%%%%%%%%%%%%%%%%%%%%%%%%%%%%%%%%%%%%%%%%%%%%%%
\begin{tcolorbox}
    (a) What is agent \( j \)'s demand, \( x^j_1(p, \omega^j_1, \omega^j_2) \) and \( x^j_2(p, \omega^j_1, \omega^j_2) \)?
\end{tcolorbox}

Solving the maximization problem:
\begin{eqnarray*}
\max_{x_1^j, x_2^j} U(x_1^j,x_2^j)&=&\sqrt{x_1^J}+\sqrt{x_2^J}\\
s.t. \quad m^j&=&p(w_1^j)+w_2^j\\
p(w_1^j)+w_2^j&>&p(x_1^j)+x_2^j\\
\end{eqnarray*}

Calculating the first order conditions:
\begin{eqnarray*}
\frac{dU}{dx_1^J}&=&\frac{1}{2\sqrt{X_1^J}}-λp=0\\
\frac{dU}{dx_2^J}&=&\frac{1}{2\sqrt{X_2^J}}-λ=0\\
\frac{dU}{dλ}&=&p(w_1^j)+w_2^j-p(x_1^j)-x_2^j=0\\
x_2^j&=&p(w_1^j)+w_2^j-p(x_1^j)\\
\end{eqnarray*}

Solving for $\lambda$:
\begin{eqnarray*}
\frac{1}{2\sqrt{X_2^J}}&=&\frac{1}{2p\sqrt{X_1^J}}\\
\sqrt{X_1^J}&=&\frac{\sqrt{X_2^J}}{p}\\
\sqrt{X_1^J}&=&(\frac{\sqrt{X_2^J}}{p})^2\\
x_1^j&=&\frac{X_2^J}{p^2}\\
x_1^j*p^2&=&x_2^j\\
\end{eqnarray*}

Substituting in the budget constraint:
\begin{eqnarray*}
x_2^j&=&p(w_1^j)+w_2^j-p(\frac{X_2^J}{p^2})\\
x_2^j&=&p(w_1^j)+w_2^j-(\frac{X_2^J}{p})\\
x_2^j+(\frac{X_2^J}{p})&=&p(w_1^j)+w_2^j\\
x_2^j&=&\frac{p(w_1^j)+w_2^j}{1+\frac{1}{p}}\\
x_2^j&=&\frac{p(w_1^j)+w_2^j}{1+\frac{1}{p}}\\
x_2^j&=&\frac{p(w_1^j)+w_2^j}{\frac{p}{p}+\frac{1}{p}}\\
x_2^j&=&\frac{p(w_1^j)+w_2^j}{\frac{p+1}{p}}\\
x_2^j&=&\frac{p(p(w_1^j)+w_2^j)}{p+1}=\frac{p^2(p(w_1^j)+w_2^j)}{p(p+1)}\\
x_1^j&=&\frac{(p(w_1^j)+w_2^j)}{p(p+1)}\\
\end{eqnarray*}

\begin{myanswerbox}
    The j's demand for good 1 is:
    \[ x^j_1(p, \omega^j_1, \omega^j_2) = \frac{(p(w_1^j)+w_2^j)}{p(p+1)} \] and for good 2 is: 
    \[ x^j_2(p, \omega^j_1, \omega^j_2) = \frac{p^2(p(w_1^j)+w_2^j)}{p(p+1)} \]
\end{myanswerbox}

%%%%%%%%%%%%%%%%%%%%%%%%%%%%%%%%%%%%%%%%%%%%%%%%%%%%%%%%%%%%%%%%%
%%%%%%%%%%%%%%%%%%%%%%%%%%%%%%%%%%%%%%%%%%%%%%%%%%%%%%%%%%%%%%%%%
\begin{tcolorbox}
    (b) Show that agent \( j \)'s indirect utility is \( v(p, x^j_1, x^j_2) = \left[ \frac{1+p}{p} (\omega^j_1 + \omega^j_2) \right]^{1/2} \).
\end{tcolorbox}

\begin{eqnarray*}
v(X_1^j,X_2^j)&=&\sqrt{\frac{(p(w_1^j)+w_2^j)}{p(p+1)}}+\sqrt{\frac{p^2(p(w_1^j)+w_2^j)}{p(p+1)}}\\
v(X_1^j,X_2^j)&=&\sqrt{\frac{(p(w_1^j)+w_2^j)}{p(p+1)}}+p\sqrt{\frac{(p(w_1^j)+w_2^j)}{p(p+1)}}\\
v(X_1^j,X_2^j)&=&(1+p)\sqrt{\frac{(p(w_1^j)+w_2^j)}{p(p+1)}}\\
v(X_1^j,X_2^j)&=&\sqrt{(1+p)^2\frac{(p(w_1^j)+w_2^j)}{p(p+1)}}\\
\end{eqnarray*}

\begin{myanswerbox}
    \begin{eqnarray*}
    v(X_1^j,X_2^j)&=&\sqrt{\frac{1+p}{p}(pw_1^j+w_2^j)}\\
    \end{eqnarray*}
\end{myanswerbox}
%%%%%%%%%%%%%%%%%%%%%%%%%%%%%%%%%%%%%%%%%%%%%%%%%%%%%%%%%%%%%%%%%
%%%%%%%%%%%%%%%%%%%%%%%%%%%%%%%%%%%%%%%%%%%%%%%%%%%%%%%%%%%%%%%%%
\begin{tcolorbox}
    (c) Equating aggregate demand and the aggregate endowments, solve for equilibrium prices.
\end{tcolorbox}

\begin{eqnarray*}
X_1&=&\sum_{j} \frac{p(w_1^j) + w_2^j}{p(p+1)} = \sum_{j} w_1^j\\
X_1&=&\sum_{j} \frac{p(w_1^j) + w_2^j}{p(p+1)} = w_1\\
X_1&=& \frac{p\sum_{j}(w_1^j) + \sum_{j}w_2^j}{p(p+1)} = w_1\\
\end{eqnarray*}

\begin{myanswerbox}
    \begin{eqnarray*}
        X_1&=& w_1\\
        X_2&=& w_2\\
    \end{eqnarray*}
\end{myanswerbox}

\begin{eqnarray*}
 \frac{p(w_1) + w_2}{p(p+1)} &=& w_1\\
 \frac{p(w_1) + w_2}{w_1} &=& p(p+1)\\
 p+\frac{w_2}{w_1} &=& p^2+p\\
\frac{w_2}{w_1} &=& p^2\\
\end{eqnarray*}

\begin{myanswerbox}
    \begin{eqnarray*}
    \sqrt\frac{w_2}{w_1} &=& p\\
    \end{eqnarray*}
\end{myanswerbox}
%%%%%%%%%%%%%%%%%%%%%%%%%%%%%%%%%%%%%%%%%%%%%%%%%%%%%%%%%%%%%%%%%
%%%%%%%%%%%%%%%%%%%%%%%%%%%%%%%%%%%%%%%%%%%%%%%%%%%%%%%%%%%%%%%%%
\begin{tcolorbox}
    (d) Show that agent \( j \) is a net seller of good 1 if
    \[
    \frac{\omega^j_1}{\omega^j_2} > \frac{\omega_1}{\omega_2}.
    \]
\end{tcolorbox}

\begin{eqnarray*}
\frac{w_2^j}{w_1^j}&<&\frac{w_2}{w_1}\\
\frac{w_2^j}{w_1^j}&<&p^2\\
x_1^j&=&\frac{(p(w_1^j)+w_2^j)}{p(p+1)}\\
x_1^jp(p+1)&=&(p(w_1^j)+w_2^j)\\
x_1^j(p^2+p)&=&(p(w_1^j)+w_2^j)\\
\frac{x_1^j(p^2+p)}{w_1^j}-p&=&\frac{w_2^j}{w_1^j}\\
\end{eqnarray*}

From that results then:


\begin{eqnarray*}
\frac{x_1^j(p^2+p)}{w_1^j}-p&<&p^2\\
\frac{x_1^j(p+1)}{w_1^j}-1&<&p\\
\frac{x_1^j(p+1)}{w_1^j}&<&p+1\\
(x_1^j)(p+1)&<&(p+1)(w_1^j)\\
x_1^j&<&w_1^j\\
\end{eqnarray*}

\begin{myanswerbox}
    Therefore, if \( \frac{\omega^j_1}{\omega^j_2} > \frac{\omega_1}{\omega_2} \), then \( x_1^j<w_1^j \), meaning that the optimal consumption of good 1 for agent $j$ is than the initial endowment, so agent $j$ is a net seller of good 1.
\end{myanswerbox}
%%%%%%%%%%%%%%%%%%%%%%%%%%%%%%%%%%%%%%%%%%%%%%%%%%%%%%%%%%%%%%%%%
%%%%%%%%%%%%%%%%%%%%%%%%%%%%%%%%%%%%%%%%%%%%%%%%%%%%%%%%%%%%%%%%%
\begin{tcolorbox}
        (e) Suppose an agent \( k \) finds a small amount of good 2, so their endowment \( \omega^k_2 \) rises a little. How does this impact the price \( p \)? Show that agent \( j \)'s utility increases if she is a net seller of good 1.
\end{tcolorbox}

If $w_2^k$ grows, $ w_2= \sum_{j} w_2^j$ will grow, and consequently, the price ($\sqrt\frac{w_2}{w_1} = p$) will increase.\\

When agent j is a net seller, it implies an increase in $w_1^j$ compared to the case when she is not a net seller, therefore her utility ($v(X_1^j,X_2^j)=\sqrt{\frac{1+p}{p}(pw_1^j+w_2^j)}$) will increase.
%%%%%%%%%%%%%%%%%%%%%%%%%%%%%%%%%%%%%%%%%%%%%%%%%%%%%%%%%%%%%%%%%